<?xml version="1.0"?>
<rdf:RDF xmlns="http://www.w3id.org/empirion#"
     xml:base="http://www.w3id.org/empirion"
     xmlns:obo="http://purl.obolibrary.org/obo/"
     xmlns:owl="http://www.w3.org/2002/07/owl#"
     xmlns:rdf="http://www.w3.org/1999/02/22-rdf-syntax-ns#"
     xmlns:xml="http://www.w3.org/XML/1998/namespace"
     xmlns:xsd="http://www.w3.org/2001/XMLSchema#"
     xmlns:rdfs="http://www.w3.org/2000/01/rdf-schema#">
    <owl:Ontology rdf:about="http://www.w3id.org/empirion"/>
    


    <!-- 
    ///////////////////////////////////////////////////////////////////////////////////////
    //
    // Object Properties
    //
    ///////////////////////////////////////////////////////////////////////////////////////
     -->

    


    <!-- http://www.w3id.org/empirion#derivedFrom -->

    <owl:ObjectProperty rdf:about="http://www.w3id.org/empirion#derivedFrom"/>
    


    <!-- http://www.w3id.org/empirion#hasResponseCharacteristics -->

    <owl:ObjectProperty rdf:about="http://www.w3id.org/empirion#hasResponseCharacteristics">
        <rdfs:comment>A set of properties for connection of Response with its Response Characteristics. Should be extended with respect to the other characteristics.</rdfs:comment>
    </owl:ObjectProperty>
    


    <!-- http://www.w3id.org/empirion#hasResponseRole -->

    <owl:ObjectProperty rdf:about="http://www.w3id.org/empirion#hasResponseRole">
        <rdfs:domain rdf:resource="http://www.cogpo.org/ontologies/CogPOver2010.owl#COGPO_00175"/>
        <rdfs:range rdf:resource="http://www.cogpo.org/ontologies/CogPOver1.owl#COGPO_00134"/>
    </owl:ObjectProperty>
    


    <!-- http://www.w3id.org/empirion#hasStimulusCharacteristics -->

    <owl:ObjectProperty rdf:about="http://www.w3id.org/empirion#hasStimulusCharacteristics">
        <rdfs:domain rdf:resource="http://www.cogpo.org/ontologies/CogPOver1.owl#COGPO_00122"/>
        <rdfs:range rdf:resource="http://www.w3id.org/empirion#StimulusCharacteristics"/>
        <rdfs:comment>A set of properties for connection of Stimulus with its Stimulus Characteristics. Should be extended with respect to the other characteristics.</rdfs:comment>
    </owl:ObjectProperty>
    


    <!-- http://www.w3id.org/empirion#hasStimulusModality -->

    <owl:ObjectProperty rdf:about="http://www.w3id.org/empirion#hasStimulusModality">
        <rdfs:subPropertyOf rdf:resource="http://www.w3id.org/empirion#hasStimulusCharacteristics"/>
        <rdfs:domain rdf:resource="http://www.cogpo.org/ontologies/CogPOver1.owl#COGPO_00122"/>
        <rdfs:range rdf:resource="http://www.cogpo.org/ontologies/CogPOver1.owl#COGPO_00124"/>
    </owl:ObjectProperty>
    


    <!-- http://www.w3id.org/empirion#hasStimulusRole -->

    <owl:ObjectProperty rdf:about="http://www.w3id.org/empirion#hasStimulusRole">
        <rdfs:domain rdf:resource="http://www.cogpo.org/ontologies/CogPOver1.owl#COGPO_00122"/>
        <rdfs:range rdf:resource="http://www.cogpo.org/ontologies/CogPOver1.owl#COGPO_00135"/>
    </owl:ObjectProperty>
    


    <!-- http://www.w3id.org/empirion#isContainedIn -->

    <owl:ObjectProperty rdf:about="http://www.w3id.org/empirion#isContainedIn">
        <rdfs:domain rdf:resource="http://www.w3id.org/empirion#Variable"/>
        <rdfs:range rdf:resource="http://rdf-vocabulary.ddialliance.org/discovery#DataFile"/>
    </owl:ObjectProperty>
    


    <!-- 
    ///////////////////////////////////////////////////////////////////////////////////////
    //
    // Classes
    //
    ///////////////////////////////////////////////////////////////////////////////////////
     -->

    


    <!-- http://bmkeg.isi.edu/ooevv/edu.isi.bmkeg.ooevv.model.scale.MeasurementScale -->

    <owl:Class rdf:about="http://bmkeg.isi.edu/ooevv/edu.isi.bmkeg.ooevv.model.scale.MeasurementScale">
        <rdfs:subClassOf rdf:resource="http://www.w3id.org/empirion#VariableSensemaker"/>
        <rdfs:comment>An abstract class (that cannot itself be instantiated) that denotes the mathematical properties of values associated with specific variables. The measurement scale denotes the data properties of the measurement but does not itself denote the quality that the variable is measuring. Each scale provides characteristics of a set of values that associated with variables.</rdfs:comment>
        <rdfs:comment>Subclasses should be imported from OoEVV.</rdfs:comment>
        <rdfs:label>MeasurementScale</rdfs:label>
    </owl:Class>
    


    <!-- http://bmkeg.isi.edu/ooevv/edu.isi.bmkeg.ooevv.model.value.MeasurementValue -->

    <owl:Class rdf:about="http://bmkeg.isi.edu/ooevv/edu.isi.bmkeg.ooevv.model.value.MeasurementValue">
        <rdfs:subClassOf rdf:resource="http://www.w3id.org/empirion#VariableSensemaker"/>
        <rdfs:comment>An abstract class denoting a value derived from a specific measurement of a specific variable.</rdfs:comment>
        <rdfs:comment>Subclasses should be imported from OoEVV.</rdfs:comment>
        <rdfs:label>MeasurementValue</rdfs:label>
    </owl:Class>
    


    <!-- http://rdf-vocabulary.ddialliance.org/discovery#DataFile -->

    <owl:Class rdf:about="http://rdf-vocabulary.ddialliance.org/discovery#DataFile">
        <rdfs:subClassOf rdf:resource="http://www.w3id.org/empirion#Data"/>
        <rdfs:comment>The class DataFile, which is also a dcmitype:Dataset, represents all the data files containing the microdata datasets.</rdfs:comment>
        <rdfs:isDefinedBy rdf:resource="http://rdf-vocabulary.ddialliance.org/discovery"/>
        <rdfs:label>Data File</rdfs:label>
    </owl:Class>
    


    <!-- http://rdf-vocabulary.ddialliance.org/discovery#Representation -->

    <owl:Class rdf:about="http://rdf-vocabulary.ddialliance.org/discovery#Representation">
        <rdfs:comment>Representation of a variable or question definition.</rdfs:comment>
        <rdfs:isDefinedBy rdf:resource="http://rdf-vocabulary.ddialliance.org/discovery"/>
        <rdfs:label>Representation</rdfs:label>
    </owl:Class>
    


    <!-- http://rdf-vocabulary.ddialliance.org/discovery#RepresentedVariable -->

    <owl:Class rdf:about="http://rdf-vocabulary.ddialliance.org/discovery#RepresentedVariable">
        <rdfs:comment>RepresentedVariables encompasse study-independent, re-usable parts of variables like occupation classification.</rdfs:comment>
        <rdfs:isDefinedBy rdf:resource="http://rdf-vocabulary.ddialliance.org/discovery"/>
        <rdfs:label>Data element</rdfs:label>
    </owl:Class>
    


    <!-- http://www.cogpo.org/ontologieButton%20Press -->

    <owl:Class rdf:about="http://www.cogpo.org/ontologieButton%20Press">
        <rdfs:subClassOf rdf:resource="http://www.cogpo.org/ontologies/CogPOver1.owl#COGPO_00136"/>
        <rdfs:comment>The class contains other subclasses that should be also imported.</rdfs:comment>
        <rdfs:label>Button Press</rdfs:label>
    </owl:Class>
    


    <!-- http://www.cogpo.org/ontologies/COGPO_00154 -->

    <owl:Class rdf:about="http://www.cogpo.org/ontologies/COGPO_00154">
        <rdfs:subClassOf rdf:resource="http://www.cogpo.org/ontologies/CogPOver2010.owl#COGPO_00177"/>
        <rdfs:label>Faces</rdfs:label>
    </owl:Class>
    


    <!-- http://www.cogpo.org/ontologies/COGPO_00162 -->

    <owl:Class rdf:about="http://www.cogpo.org/ontologies/COGPO_00162">
        <rdfs:subClassOf rdf:resource="http://www.w3id.org/empirion#Character"/>
        <rdfs:label>Digits</rdfs:label>
    </owl:Class>
    


    <!-- http://www.cogpo.org/ontologies/COGPO_00163 -->

    <owl:Class rdf:about="http://www.cogpo.org/ontologies/COGPO_00163">
        <rdfs:subClassOf rdf:resource="http://www.w3id.org/empirion#Character"/>
        <rdfs:label>Letters</rdfs:label>
    </owl:Class>
    


    <!-- http://www.cogpo.org/ontologies/COGPO_00169 -->

    <owl:Class rdf:about="http://www.cogpo.org/ontologies/COGPO_00169">
        <rdfs:subClassOf rdf:resource="http://www.w3id.org/empirion#Character"/>
        <rdfs:comment>A sound or a combination of sounds, or its representation in writing or printing, that symbolizes and communicates a meaning and may consist of a single morpheme or of a combination of morphemes.</rdfs:comment>
        <rdfs:isDefinedBy>The American Heritage  Dictionary of the English Language, Fourth Edition. Retrieved April 16, 2010, from Dictionary.com website: http://dictionary.reference.com/browse/word</rdfs:isDefinedBy>
        <rdfs:label>Words</rdfs:label>
    </owl:Class>
    


    <!-- http://www.cogpo.org/ontologies/COGPO_00172 -->

    <owl:Class rdf:about="http://www.cogpo.org/ontologies/COGPO_00172">
        <rdfs:subClassOf rdf:resource="http://www.cogpo.org/ontologies/CogPOver2010.owl#COGPO_00177"/>
        <rdfs:comment>A representation or image that is painted, drawn, photographed, or otherwise rendered on a flat surface.</rdfs:comment>
        <rdfs:isDefinedBy>The American Heritage  Dictionary of the English Language, Fourth Edition. Retrieved April 16, 2010, from Dictionary.com website: http://dictionary.reference.com/browse/pictures</rdfs:isDefinedBy>
        <rdfs:label>Pictures</rdfs:label>
    </owl:Class>
    


    <!-- http://www.cogpo.org/ontologies/CogPOver1.owl#COGPO_00028 -->

    <owl:Class rdf:about="http://www.cogpo.org/ontologies/CogPOver1.owl#COGPO_00028">
        <rdfs:subClassOf rdf:resource="http://www.w3id.org/empirion#ExperimentCharacteristic"/>
        <rdfs:comment>Instructions are the information-bearing entity that sets up the rules for desired behavior from the subjects. An explicit direction that guides the behavior of the subject during the experimental conditions. 
Instructions serve the function that they lay out what the response behaviors should be for any set of stimuli in the experiment.</rdfs:comment>
        <rdfs:comment>The class has subclasses that should be imported.</rdfs:comment>
        <rdfs:label>Instructions</rdfs:label>
    </owl:Class>
    


    <!-- http://www.cogpo.org/ontologies/CogPOver1.owl#COGPO_00049 -->

    <owl:Class rdf:about="http://www.cogpo.org/ontologies/CogPOver1.owl#COGPO_00049">
        <rdfs:subClassOf rdf:resource="http://www.w3id.org/empirion#CognitiveScienceExperimentProcedure"/>
        <rdfs:comment>The class contains other subclasses that should be also imported.</rdfs:comment>
        <rdfs:label>Behavioral Experimental Paradigm</rdfs:label>
    </owl:Class>
    


    <!-- http://www.cogpo.org/ontologies/CogPOver1.owl#COGPO_00059 -->

    <owl:Class rdf:about="http://www.cogpo.org/ontologies/CogPOver1.owl#COGPO_00059">
        <rdfs:subClassOf rdf:resource="http://www.cogpo.org/ontologies/CogPOver1.owl#COGPO_00049"/>
        <rdfs:label>Flanker Task Paradigm</rdfs:label>
    </owl:Class>
    


    <!-- http://www.cogpo.org/ontologies/CogPOver1.owl#COGPO_00119 -->

    <owl:Class rdf:about="http://www.cogpo.org/ontologies/CogPOver1.owl#COGPO_00119">
        <rdfs:subClassOf rdf:resource="http://www.w3id.org/empirion#ResponseCharacteristic"/>
        <rdfs:comment>How the response to the stimulus was given (i.e., with hand, or more pricisely with right middle finger). The CogPO creators used corresponding FMA ontology classes.</rdfs:comment>
        <rdfs:label>Response Modality</rdfs:label>
    </owl:Class>
    


    <!-- http://www.cogpo.org/ontologies/CogPOver1.owl#COGPO_00122 -->

    <owl:Class rdf:about="http://www.cogpo.org/ontologies/CogPOver1.owl#COGPO_00122">
        <rdfs:subClassOf rdf:resource="http://www.w3id.org/empirion#Variable"/>
        <rdfs:comment>The  object or set of objects, internal or external to the subject, which is intended to generate either an overt or covert response in the subject as part of an experimental condition.</rdfs:comment>
        <rdfs:label>Stimulus</rdfs:label>
    </owl:Class>
    


    <!-- http://www.cogpo.org/ontologies/CogPOver1.owl#COGPO_00124 -->

    <owl:Class rdf:about="http://www.cogpo.org/ontologies/CogPOver1.owl#COGPO_00124">
        <rdfs:subClassOf rdf:resource="http://www.w3id.org/empirion#StimulusCharacteristics"/>
        <rdfs:comment>The class contains other subclasses that should be also imported.</rdfs:comment>
        <rdfs:label>Stimulus Modality</rdfs:label>
    </owl:Class>
    


    <!-- http://www.cogpo.org/ontologies/CogPOver1.owl#COGPO_00134 -->

    <owl:Class rdf:about="http://www.cogpo.org/ontologies/CogPOver1.owl#COGPO_00134">
        <rdfs:subClassOf rdf:resource="http://www.w3id.org/empirion#Variable"/>
        <rdfs:comment>The role of response is attributed to the overt or covert behavior which is elicited from the subject in an experimental condition.</rdfs:comment>
        <rdfs:label>Response Role</rdfs:label>
    </owl:Class>
    


    <!-- http://www.cogpo.org/ontologies/CogPOver1.owl#COGPO_00135 -->

    <owl:Class rdf:about="http://www.cogpo.org/ontologies/CogPOver1.owl#COGPO_00135">
        <rdfs:subClassOf rdf:resource="http://www.w3id.org/empirion#Variable"/>
        <rdfs:comment>The role of a stimulus in a behavioral experiment is attributed to the object(s) which are presented to the subject in a controlled manner in the context of the experiment.</rdfs:comment>
        <rdfs:label>Stimulus Role</rdfs:label>
    </owl:Class>
    


    <!-- http://www.cogpo.org/ontologies/CogPOver1.owl#COGPO_00136 -->

    <owl:Class rdf:about="http://www.cogpo.org/ontologies/CogPOver1.owl#COGPO_00136">
        <rdfs:subClassOf rdf:resource="http://www.cogpo.org/ontologies/CogPOver2010.owl#COGPO_00175"/>
        <rdfs:comment>An overt response is a Response made with a body part that is externally observable by others.</rdfs:comment>
        <rdfs:comment>The class contains other subclasses that should be also imported.</rdfs:comment>
        <rdfs:label>Overt Response</rdfs:label>
    </owl:Class>
    


    <!-- http://www.cogpo.org/ontologies/CogPOver2010.owl#COGPO_00175 -->

    <owl:Class rdf:about="http://www.cogpo.org/ontologies/CogPOver2010.owl#COGPO_00175">
        <rdfs:subClassOf rdf:resource="http://www.w3id.org/empirion#Variable"/>
        <rdfs:comment>The overt or covert behavior which is elicited from the subject in an experimental condition.</rdfs:comment>
        <rdfs:label>Response</rdfs:label>
    </owl:Class>
    


    <!-- http://www.cogpo.org/ontologies/CogPOver2010.owl#COGPO_00176 -->

    <owl:Class rdf:about="http://www.cogpo.org/ontologies/CogPOver2010.owl#COGPO_00176">
        <rdfs:subClassOf rdf:resource="http://www.cogpo.org/ontologies/CogPOver2010.owl#COGPO_00175"/>
        <rdfs:comment>A covert response is a Response made internal to the body, which is unobservable by external viewers.</rdfs:comment>
        <rdfs:label>Covert Response</rdfs:label>
    </owl:Class>
    


    <!-- http://www.cogpo.org/ontologies/CogPOver2010.owl#COGPO_00177 -->

    <owl:Class rdf:about="http://www.cogpo.org/ontologies/CogPOver2010.owl#COGPO_00177">
        <rdfs:subClassOf rdf:resource="http://www.cogpo.org/ontologies/CogPOver1.owl#COGPO_00122"/>
        <rdfs:comment>A stimulus which exists at least in part externally to the subject--e.g., a flashing checkerboard, a drop of juice, a set of digits, an electrical charge, etc.</rdfs:comment>
        <rdfs:comment>The class contains other subclasses that should be also imported.</rdfs:comment>
        <rdfs:label>Explicit Stimulus</rdfs:label>
    </owl:Class>
    


    <!-- http://www.cogpo.org/ontologies/CogPOver2010.owl#COGPO_00178 -->

    <owl:Class rdf:about="http://www.cogpo.org/ontologies/CogPOver2010.owl#COGPO_00178">
        <rdfs:subClassOf rdf:resource="http://www.cogpo.org/ontologies/CogPOver1.owl#COGPO_00122"/>
        <rdfs:comment>A stimulus generated internally by the subject--e.g., resting with eyes closed, imaging a scene, re-living an experience, etc</rdfs:comment>
        <rdfs:label>Implicit Stimulus</rdfs:label>
    </owl:Class>
    


    <!-- http://www.w3id.org/empirion#Character -->

    <owl:Class rdf:about="http://www.w3id.org/empirion#Character">
        <rdfs:subClassOf rdf:resource="http://www.cogpo.org/ontologies/CogPOver2010.owl#COGPO_00177"/>
        <rdfs:comment>Stimulus consisted of the written signs (letters, numbers, signs, etc.)</rdfs:comment>
    </owl:Class>
    


    <!-- http://www.w3id.org/empirion#CognitiveScienceExperimentProcedure -->

    <owl:Class rdf:about="http://www.w3id.org/empirion#CognitiveScienceExperimentProcedure">
        <rdfs:subClassOf rdf:resource="http://www.w3id.org/empirion#ExperimentProcedure"/>
    </owl:Class>
    


    <!-- http://www.w3id.org/empirion#CueStimulus -->

    <owl:Class rdf:about="http://www.w3id.org/empirion#CueStimulus">
        <rdfs:subClassOf rdf:resource="http://www.cogpo.org/ontologies/CogPOver1.owl#COGPO_00135"/>
    </owl:Class>
    


    <!-- http://www.w3id.org/empirion#Data -->

    <owl:Class rdf:about="http://www.w3id.org/empirion#Data">
        <rdfs:comment>Representation of the data in material world.</rdfs:comment>
        <rdfs:label>Data</rdfs:label>
    </owl:Class>
    


    <!-- http://www.w3id.org/empirion#DerivedVariable -->

    <owl:Class rdf:about="http://www.w3id.org/empirion#DerivedVariable">
        <rdfs:subClassOf rdf:resource="http://rdf-vocabulary.ddialliance.org/discovery#RepresentedVariable"/>
        <rdfs:subClassOf>
            <owl:Restriction>
                <owl:onProperty rdf:resource="http://www.w3id.org/empirion#derivedFrom"/>
                <owl:someValuesFrom rdf:resource="http://www.w3id.org/empirion#RawVariable"/>
            </owl:Restriction>
        </rdfs:subClassOf>
        <rdfs:label>A data element that was derived from other data element or somehow transformed. For example, denotion of the answer as correct or erroneous.</rdfs:label>
        <rdfs:label>Derived Variable</rdfs:label>
    </owl:Class>
    


    <!-- http://www.w3id.org/empirion#ExperementBlockCharacteristics -->

    <owl:Class rdf:about="http://www.w3id.org/empirion#ExperementBlockCharacteristics">
        <rdfs:subClassOf rdf:resource="http://www.w3id.org/empirion#ExperimentPartCharacteristic"/>
        <rdfs:comment>&quot;Block design&quot; is a type of research study in which participants are divided into relatively homogeneous subsets (blocks) from which they are assigned to the experimental or treatment conditions. For example, in a simple block design to evaluate the efficacy of several antidepressants, participants with similar pretest depression scores might be grouped into homogeneous blocks and then assigned to receive different medications. The purpose of a block design is to ensure that a characteristic of the study participants that is related to the target outcome (i.e., a covariate) is distributed equally across treatment conditions.</rdfs:comment>
        <rdfs:comment>An experiment may consist of several parts which are often called &quot;blocks&quot;.</rdfs:comment>
        <rdfs:isDefinedBy>https://dictionary.apa.org/block-design</rdfs:isDefinedBy>
    </owl:Class>
    


    <!-- http://www.w3id.org/empirion#ExperementBlockNumber -->

    <owl:Class rdf:about="http://www.w3id.org/empirion#ExperementBlockNumber">
        <rdfs:subClassOf rdf:resource="http://www.w3id.org/empirion#ExperementBlockCharacteristics"/>
        <rdfs:comment>Number of the experiment block.</rdfs:comment>
    </owl:Class>
    


    <!-- http://www.w3id.org/empirion#ExperementTrialCharacterictics -->

    <owl:Class rdf:about="http://www.w3id.org/empirion#ExperementTrialCharacterictics">
        <rdfs:subClassOf rdf:resource="http://www.w3id.org/empirion#ExperimentPartCharacteristic"/>
        <rdfs:comment>Trial. In testing, conditioning, or other experimentation, a single performance of a given task (e.g., one run through a maze) or a single presentation of a stimulus (e.g., one viewing of an ordered list of three-letter words).</rdfs:comment>
        <rdfs:isDefinedBy>https://dictionary.apa.org/trial</rdfs:isDefinedBy>
    </owl:Class>
    


    <!-- http://www.w3id.org/empirion#ExperementTrialNumber -->

    <owl:Class rdf:about="http://www.w3id.org/empirion#ExperementTrialNumber">
        <rdfs:subClassOf rdf:resource="http://www.w3id.org/empirion#ExperementTrialCharacterictics"/>
        <rdfs:comment>Number of the trial.</rdfs:comment>
    </owl:Class>
    


    <!-- http://www.w3id.org/empirion#ExperimentCharacteristic -->

    <owl:Class rdf:about="http://www.w3id.org/empirion#ExperimentCharacteristic">
        <rdfs:subClassOf rdf:resource="http://www.w3id.org/empirion#Metadata"/>
        <rdfs:comment>Characteristics of an experiment. Experiment is a series of observations conducted under controlled conditions to study a relationship with the purpose of drawing causal inferences about that relationship. An experiment involves the manipulation of an independent variable, the measurement of a dependent variable, and the exposure of various participants to one or more of the conditions being studied. Random selection of participants and their random assignment to conditions also are necessary in experiments. —experimental adj.</rdfs:comment>
        <rdfs:isDefinedBy>https://dictionary.apa.org/experiment</rdfs:isDefinedBy>
    </owl:Class>
    


    <!-- http://www.w3id.org/empirion#ExperimentNumber -->

    <owl:Class rdf:about="http://www.w3id.org/empirion#ExperimentNumber">
        <rdfs:subClassOf rdf:resource="http://www.w3id.org/empirion#ExperimentCharacteristic"/>
        <rdfs:comment>Number or ID (identifier) of the experiment in the connected paper or report.</rdfs:comment>
    </owl:Class>
    


    <!-- http://www.w3id.org/empirion#ExperimentPartCharacteristic -->

    <owl:Class rdf:about="http://www.w3id.org/empirion#ExperimentPartCharacteristic">
        <rdfs:subClassOf rdf:resource="http://www.w3id.org/empirion#Variable"/>
        <rdfs:comment>Characteristics of the parts of the experiment.</rdfs:comment>
    </owl:Class>
    


    <!-- http://www.w3id.org/empirion#ExperimentProcedure -->

    <owl:Class rdf:about="http://www.w3id.org/empirion#ExperimentProcedure">
        <rdfs:subClassOf rdf:resource="http://www.w3id.org/empirion#ExperimentCharacteristic"/>
    </owl:Class>
    


    <!-- http://www.w3id.org/empirion#ExperimentSetting -->

    <owl:Class rdf:about="http://www.w3id.org/empirion#ExperimentSetting">
        <rdfs:subClassOf rdf:resource="http://www.w3id.org/empirion#ExperimentCharacteristic"/>
        <rdfs:comment>Characteristics of the evironment in which the experiment was conducted.</rdfs:comment>
    </owl:Class>
    


    <!-- http://www.w3id.org/empirion#LicenseFile -->

    <owl:Class rdf:about="http://www.w3id.org/empirion#LicenseFile">
        <rdfs:subClassOf rdf:resource="http://www.w3id.org/empirion#MetadataFile"/>
        <rdfs:label>License File</rdfs:label>
    </owl:Class>
    


    <!-- http://www.w3id.org/empirion#MaskStimulus -->

    <owl:Class rdf:about="http://www.w3id.org/empirion#MaskStimulus">
        <rdfs:subClassOf rdf:resource="http://www.cogpo.org/ontologies/CogPOver1.owl#COGPO_00135"/>
    </owl:Class>
    


    <!-- http://www.w3id.org/empirion#MeasurementUnit -->

    <owl:Class rdf:about="http://www.w3id.org/empirion#MeasurementUnit">
        <rdfs:subClassOf rdf:resource="http://www.w3id.org/empirion#VariableSensemaker"/>
        <rdfs:comment>Similar to GSIM Unit Type and iao measurement unit label.</rdfs:comment>
    </owl:Class>
    


    <!-- http://www.w3id.org/empirion#Metadata -->

    <owl:Class rdf:about="http://www.w3id.org/empirion#Metadata">
        <rdfs:label>Metadata</rdfs:label>
    </owl:Class>
    


    <!-- http://www.w3id.org/empirion#MetadataFile -->

    <owl:Class rdf:about="http://www.w3id.org/empirion#MetadataFile">
        <rdfs:subClassOf rdf:resource="http://www.w3id.org/empirion#Data"/>
        <rdfs:comment>The files with metadata about the data set.</rdfs:comment>
        <rdfs:label>Metadata File</rdfs:label>
    </owl:Class>
    


    <!-- http://www.w3id.org/empirion#PrimeResponse -->

    <owl:Class rdf:about="http://www.w3id.org/empirion#PrimeResponse">
        <rdfs:subClassOf rdf:resource="http://www.cogpo.org/ontologies/CogPOver1.owl#COGPO_00134"/>
    </owl:Class>
    


    <!-- http://www.w3id.org/empirion#PrimeStimulus -->

    <owl:Class rdf:about="http://www.w3id.org/empirion#PrimeStimulus">
        <rdfs:subClassOf rdf:resource="http://www.cogpo.org/ontologies/CogPOver1.owl#COGPO_00135"/>
    </owl:Class>
    


    <!-- http://www.w3id.org/empirion#ProcedureSpecificStimulusCharacteristic -->

    <owl:Class rdf:about="http://www.w3id.org/empirion#ProcedureSpecificStimulusCharacteristic">
        <rdfs:subClassOf rdf:resource="http://www.w3id.org/empirion#StimulusCharacteristics"/>
    </owl:Class>
    


    <!-- http://www.w3id.org/empirion#RawVariable -->

    <owl:Class rdf:about="http://www.w3id.org/empirion#RawVariable">
        <rdfs:subClassOf rdf:resource="http://rdf-vocabulary.ddialliance.org/discovery#RepresentedVariable"/>
        <rdfs:comment>A data element thet was obtained directly from research participant&apos;s answer without any transformation. For example, measurement of reaction time or answer to the question about the age.</rdfs:comment>
        <rdfs:label>Raw Variable</rdfs:label>
    </owl:Class>
    


    <!-- http://www.w3id.org/empirion#ResponseAccuracy -->

    <owl:Class rdf:about="http://www.w3id.org/empirion#ResponseAccuracy">
        <rdfs:subClassOf rdf:resource="http://www.w3id.org/empirion#ResponseCharacteristic"/>
        <rdfs:comment>Accuracy is a measure of performance on a task, usually defined as the proportion of correct responses.</rdfs:comment>
        <rdfs:isDefinedBy>https://dictionary.apa.org/accuracy</rdfs:isDefinedBy>
    </owl:Class>
    


    <!-- http://www.w3id.org/empirion#ResponseCharacteristic -->

    <owl:Class rdf:about="http://www.w3id.org/empirion#ResponseCharacteristic">
        <rdfs:subClassOf rdf:resource="http://www.w3id.org/empirion#Variable"/>
        <rdfs:comment>Characteristics of the response. Responce is any glandular, muscular, neural, or other reaction to a stimulus. A response is a clearly defined, measurable unit of behavior discussed in terms of its result (e.g., pressing a lever, indicating yes vs. no on a survey item) or its physical characteristics (e.g., raising an arm).</rdfs:comment>
        <rdfs:isDefinedBy>https://dictionary.apa.org/response</rdfs:isDefinedBy>
    </owl:Class>
    


    <!-- http://www.w3id.org/empirion#ResponseTime -->

    <owl:Class rdf:about="http://www.w3id.org/empirion#ResponseTime">
        <rdfs:subClassOf rdf:resource="http://www.w3id.org/empirion#ResponseCharacteristic"/>
        <rdfs:comment>Reaction time is the time that elapses between the onset or presentation of a stimulus and the occurrence of a specific response to that stimulus. There are several types, including simple reaction time and choice reaction time. Reaction time can be used to assess various psychological constructs. To assess negative affect, for example, a researcher might measure the time between presentation of various words with emotional connotations and a participant’s indication that each word is either “positive” or “negative.” Also called response latency; response time.</rdfs:comment>
        <rdfs:isDefinedBy>https://dictionary.apa.org/reaction-time</rdfs:isDefinedBy>
    </owl:Class>
    


    <!-- http://www.w3id.org/empirion#StimulusCharacteristics -->

    <owl:Class rdf:about="http://www.w3id.org/empirion#StimulusCharacteristics">
        <rdfs:subClassOf rdf:resource="http://www.w3id.org/empirion#Variable"/>
        <rdfs:comment>Characteristics of Stimulus. Distal stimulus in perception, the actual object in the environment that stimulates or acts on a sense organ.</rdfs:comment>
        <rdfs:isDefinedBy>https://dictionary.apa.org/distal-stimulus</rdfs:isDefinedBy>
    </owl:Class>
    


    <!-- http://www.w3id.org/empirion#StimulusColor -->

    <owl:Class rdf:about="http://www.w3id.org/empirion#StimulusColor">
        <rdfs:subClassOf rdf:resource="http://www.w3id.org/empirion#StimulusCharacteristics"/>
        <rdfs:comment>Color of the stimulus.</rdfs:comment>
    </owl:Class>
    


    <!-- http://www.w3id.org/empirion#StimulusCongruence -->

    <owl:Class rdf:about="http://www.w3id.org/empirion#StimulusCongruence">
        <rdfs:subClassOf rdf:resource="http://www.w3id.org/empirion#ProcedureSpecificStimulusCharacteristic"/>
        <rdfs:comment>Congruence of the ratio of the side parts of the stimulus (distractors or flankers) to the Central (target). in the Flanker problem fffgffff is a non congruent stimulus and ffffffff is congruent.</rdfs:comment>
    </owl:Class>
    


    <!-- http://www.w3id.org/empirion#StimulusDescription -->

    <owl:Class rdf:about="http://www.w3id.org/empirion#StimulusDescription">
        <rdfs:subClassOf rdf:resource="http://www.w3id.org/empirion#StimulusCharacteristics"/>
        <rdfs:comment>Description of the stimulus.</rdfs:comment>
    </owl:Class>
    


    <!-- http://www.w3id.org/empirion#StimulusFile -->

    <owl:Class rdf:about="http://www.w3id.org/empirion#StimulusFile">
        <rdfs:subClassOf rdf:resource="http://www.w3id.org/empirion#Data"/>
        <rdfs:comment>Path to the image or content.</rdfs:comment>
        <rdfs:label>Stimulus File</rdfs:label>
    </owl:Class>
    


    <!-- http://www.w3id.org/empirion#StimulusIdentificator -->

    <owl:Class rdf:about="http://www.w3id.org/empirion#StimulusIdentificator">
        <rdfs:subClassOf rdf:resource="http://www.w3id.org/empirion#StimulusCharacteristics"/>
        <rdfs:comment>Identificator of the stimulus. (ID)</rdfs:comment>
    </owl:Class>
    


    <!-- http://www.w3id.org/empirion#StimulusNumber -->

    <owl:Class rdf:about="http://www.w3id.org/empirion#StimulusNumber">
        <rdfs:subClassOf rdf:resource="http://www.w3id.org/empirion#StimulusCharacteristics"/>
        <rdfs:comment>Number of the stimulus.</rdfs:comment>
    </owl:Class>
    


    <!-- http://www.w3id.org/empirion#StimulusPosition -->

    <owl:Class rdf:about="http://www.w3id.org/empirion#StimulusPosition">
        <rdfs:subClassOf rdf:resource="http://www.w3id.org/empirion#StimulusCharacteristics"/>
        <rdfs:comment>Position of stimulus parts.</rdfs:comment>
    </owl:Class>
    


    <!-- http://www.w3id.org/empirion#StimulusSize -->

    <owl:Class rdf:about="http://www.w3id.org/empirion#StimulusSize">
        <rdfs:subClassOf rdf:resource="http://www.w3id.org/empirion#StimulusCharacteristics"/>
        <rdfs:comment>Size of the stimulus.</rdfs:comment>
    </owl:Class>
    


    <!-- http://www.w3id.org/empirion#StimulusValence -->

    <owl:Class rdf:about="http://www.w3id.org/empirion#StimulusValence">
        <rdfs:subClassOf rdf:resource="http://www.w3id.org/empirion#ProcedureSpecificStimulusCharacteristic"/>
        <rdfs:comment>Valence of the stimulus (positive or negative).</rdfs:comment>
    </owl:Class>
    


    <!-- http://www.w3id.org/empirion#StimulusVisualCharacteristics -->

    <owl:Class rdf:about="http://www.w3id.org/empirion#StimulusVisualCharacteristics">
        <rdfs:subClassOf rdf:resource="http://www.w3id.org/empirion#StimulusCharacteristics"/>
    </owl:Class>
    


    <!-- http://www.w3id.org/empirion#SubjectAge -->

    <owl:Class rdf:about="http://www.w3id.org/empirion#SubjectAge">
        <rdfs:subClassOf rdf:resource="http://www.w3id.org/empirion#SubjectIntrinsicCharasteristics"/>
        <rdfs:comment>Age of the subject. Age is the amount of time that has passed since an organism’s birth; that is, an individual’s chronological age. Compare gestational age.</rdfs:comment>
        <rdfs:isDefinedBy>https://dictionary.apa.org/age</rdfs:isDefinedBy>
    </owl:Class>
    


    <!-- http://www.w3id.org/empirion#SubjectCharacteristic -->

    <owl:Class rdf:about="http://www.w3id.org/empirion#SubjectCharacteristic">
        <rdfs:subClassOf rdf:resource="http://www.w3id.org/empirion#Variable"/>
        <rdfs:comment>Characteristics of the subjects. Subjecs is generally, the individual human or nonhuman animal that takes part in an experiment or research study and whose responses or performance are reported or evaluated; less frequently, the “subject” may also be an institution, group, or other entity. Many now recommend that the term participant be used for humans, considering the word subject to be depersonalizing and to imply passivity and submissiveness on the part of the experimentee.</rdfs:comment>
        <rdfs:isDefinedBy>https://dictionary.apa.org/subject</rdfs:isDefinedBy>
    </owl:Class>
    


    <!-- http://www.w3id.org/empirion#SubjectExperimentalCharasteristics -->

    <owl:Class rdf:about="http://www.w3id.org/empirion#SubjectExperimentalCharasteristics">
        <rdfs:subClassOf rdf:resource="http://www.w3id.org/empirion#SubjectCharacteristic"/>
        <rdfs:comment>Charaxteristics of the subject that are dependent on the experiment procedure.</rdfs:comment>
    </owl:Class>
    


    <!-- http://www.w3id.org/empirion#SubjectGroup -->

    <owl:Class rdf:about="http://www.w3id.org/empirion#SubjectGroup">
        <rdfs:subClassOf rdf:resource="http://www.w3id.org/empirion#SubjectExperimentalCharasteristics"/>
        <rdfs:comment>Designation of the group that the subject belongs to. Group in research denotes a collection of participants who all experience the same experimental conditions and whose responses are to be compared to the responses of one or more other collections of research participants.</rdfs:comment>
        <rdfs:isDefinedBy>https://dictionary.apa.org/group</rdfs:isDefinedBy>
    </owl:Class>
    


    <!-- http://www.w3id.org/empirion#SubjectHandedness -->

    <owl:Class rdf:about="http://www.w3id.org/empirion#SubjectHandedness">
        <rdfs:subClassOf rdf:resource="http://www.w3id.org/empirion#SubjectIntrinsicCharasteristics"/>
        <rdfs:comment>Handedness of the subject. Handedness is the consistent use of one hand rather than the other in performing certain tasks. The preference usually is related to a dominance effect of the motor cortex on the opposite side of the body. Also called hand dominance; manual dominance. See cerebral dominance; laterality; left-handedness; right-handedness.</rdfs:comment>
        <rdfs:isDefinedBy>https://dictionary.apa.org/handedness</rdfs:isDefinedBy>
    </owl:Class>
    


    <!-- http://www.w3id.org/empirion#SubjectIntrinsicCharasteristics -->

    <owl:Class rdf:about="http://www.w3id.org/empirion#SubjectIntrinsicCharasteristics">
        <rdfs:subClassOf rdf:resource="http://www.w3id.org/empirion#SubjectCharacteristic"/>
        <rdfs:comment>Charasteristics of the subject that are inherent in the subject and are not dependent on the experiment procedure.</rdfs:comment>
    </owl:Class>
    


    <!-- http://www.w3id.org/empirion#SubjectNumber -->

    <owl:Class rdf:about="http://www.w3id.org/empirion#SubjectNumber">
        <rdfs:subClassOf rdf:resource="http://www.w3id.org/empirion#SubjectExperimentalCharasteristics"/>
        <rdfs:comment>Number or ID (identifier) of the subject.</rdfs:comment>
    </owl:Class>
    


    <!-- http://www.w3id.org/empirion#SubjectSex -->

    <owl:Class rdf:about="http://www.w3id.org/empirion#SubjectSex">
        <rdfs:subClassOf rdf:resource="http://www.w3id.org/empirion#SubjectIntrinsicCharasteristics"/>
        <rdfs:comment>Sex of the subject. Sex is the traits that distinguish between males and females. Sex refers especially to physical and biological traits, whereas gender refers especially to social or cultural traits, although the distinction between the two terms is not regularly observed.</rdfs:comment>
        <rdfs:isDefinedBy>https://dictionary.apa.org/sex</rdfs:isDefinedBy>
    </owl:Class>
    


    <!-- http://www.w3id.org/empirion#TargetResponse -->

    <owl:Class rdf:about="http://www.w3id.org/empirion#TargetResponse">
        <rdfs:subClassOf rdf:resource="http://www.cogpo.org/ontologies/CogPOver1.owl#COGPO_00134"/>
    </owl:Class>
    


    <!-- http://www.w3id.org/empirion#TargetStimulus -->

    <owl:Class rdf:about="http://www.w3id.org/empirion#TargetStimulus">
        <rdfs:subClassOf rdf:resource="http://www.cogpo.org/ontologies/CogPOver1.owl#COGPO_00135"/>
    </owl:Class>
    


    <!-- http://www.w3id.org/empirion#ValueDomain -->

    <owl:Class rdf:about="http://www.w3id.org/empirion#ValueDomain">
        <rdfs:subClassOf rdf:resource="http://www.w3id.org/empirion#VariableSensemaker"/>
        <rdfs:comment>Similar to GSIM Value Domain: The permitted range of values for a characteristic of a variable.</rdfs:comment>
        <rdfs:isDefinedBy>Codifications also count ad value domains.</rdfs:isDefinedBy>
        <rdfs:isDefinedBy>https://statswiki.unece.org/display/GSIMclick/Value+Domain</rdfs:isDefinedBy>
    </owl:Class>
    


    <!-- http://www.w3id.org/empirion#Variable -->

    <owl:Class rdf:about="http://www.w3id.org/empirion#Variable">
        <rdfs:comment>Variables provide a definition of the column in a rectangular data file. Variable is a characteristic of a unit being observed. A variable might be the answer of a question, have an administrative source, or be derived from other variables.</rdfs:comment>
        <rdfs:isDefinedBy rdf:resource="http://rdf-vocabulary.ddialliance.org/discovery"/>
        <rdfs:label>Variable</rdfs:label>
    </owl:Class>
    


    <!-- http://www.w3id.org/empirion#VariableDescription -->

    <owl:Class rdf:about="http://www.w3id.org/empirion#VariableDescription">
        <rdfs:subClassOf rdf:resource="http://www.w3id.org/empirion#MetadataFile"/>
        <rdfs:comment>The file with human readable description of the variables in the data set. Often named Codebook or ReadMe.</rdfs:comment>
        <rdfs:label>Variable Description</rdfs:label>
    </owl:Class>
    


    <!-- http://www.w3id.org/empirion#VariableSensemaker -->

    <owl:Class rdf:about="http://www.w3id.org/empirion#VariableSensemaker">
        <rdfs:subClassOf rdf:resource="http://www.w3id.org/empirion#Metadata"/>
        <rdfs:comment>This class is temporary storage for the variables&apos; characteristics that are not in the data set itself but are needed for the data correct interpretation.</rdfs:comment>
    </owl:Class>
</rdf:RDF>



<!-- Generated by the OWL API (version 4.5.9.2019-02-01T07:24:44Z) https://github.com/owlcs/owlapi -->

